HOL_To_IMP_Minus/Refinements/HOL_To_IMP_Minus_Primitives.thy
@@ -3,7 +3,7 @@ theory HOL_To_IMP_Minus_Primitives
   imports
     HOL_To_IMP_Minus_Methods
 begin
-term tailcall_to_IMP_Minus
+
 locale HOL_To_IMP_Minus =
   notes neq0_conv[iff del, symmetric, iff]
 begin
@@ -27,11 +27,7 @@ declare_compiled_const True
   argument_registers
   compiled "tailcall_to_IMP_Minus true_IMP_tailcall"
 
-
-HOL_To_IMP_Minus_func_correct true_nat
-  apply preprocess_HOL_To_IMP_Minus_func_correct
-  apply (start_run_finish true_nat_def)
-  done
+HOL_To_IMP_Minus_func_correct true_nat by (cooker HOL_eqs = true_nat_def)
 
 lemma true_nat_eq_one[simp]: "true_nat = 1"
   unfolding true_nat_def by simp
@@ -48,10 +44,7 @@ declare_compiled_const False
   argument_registers
   compiled "tailcall_to_IMP_Minus false_IMP_tailcall"
 
-HOL_To_IMP_Minus_func_correct false_nat
-  apply preprocess_HOL_To_IMP_Minus_func_correct
-  apply (start_run_finish false_nat_def)
-  done
+HOL_To_IMP_Minus_func_correct false_nat by (cooker HOL_eqs = false_nat_def)
 
 lemma false_nat_eq_one[simp]: "false_nat = 0"
   unfolding false_nat_def by simp
@@ -63,10 +56,7 @@ definition "id_nat x \<equiv> (x :: nat)"
 
 compile_nat id_nat_def basename id
 
-HOL_To_IMP_Minus_func_correct id_nat
-  apply preprocess_HOL_To_IMP_Minus_func_correct
-  apply (start_run_finish id_nat_def)
-  done
+HOL_To_IMP_Minus_func_correct id_nat by (cooker HOL_eqs = id_nat_def)
 
 lemma id_nat_eq_id[simp]: "id_nat = id"
   unfolding id_nat_def by (rule ext) simp
@@ -89,7 +79,7 @@ definition "eq_nat (n :: nat) m \<equiv> nat_of_bool (n = m)"
 context includes com_syntax no_com'_syntax
 begin
 
-definition [compiled_const_defs add]:
+definition [compiled_const_defs]:
   "eq_IMP \<equiv>
     ''eq_x_Sub_y'' ::= (V ''eq_x'' \<ominus> V ''eq_y'');;
     ''eq_y_Sub_x'' ::= (V ''eq_y'' \<ominus> V ''eq_x'');;
@@ -125,48 +115,46 @@ declare_compiled_const HOL.Not
   argument_registers "not_n"
   compiled "tailcall_to_IMP_Minus not_IMP_tailcall"
 
-HOL_To_IMP_Minus_func_correct not_nat
-  apply preprocess_HOL_To_IMP_Minus_func_correct
-  apply (start_run_finish not_nat_def)
-  done
+HOL_To_IMP_Minus_func_correct not_nat by (cooker HOL_eqs = not_nat_def)
 
 lemma not_nat_eq_nat_of_bool_eq_false[simp]: "not_nat n = nat_of_bool (n = false_nat)"
   unfolding not_nat_def by simp
 
-definition [simp]: "plus_nat (x :: nat) y \<equiv> x + y"
-definition [simp]: "minus_nat (x :: nat) y \<equiv> x - y"
+definition "add_nat (x :: nat) y \<equiv> x + y"
+definition "sub_nat (x :: nat) y \<equiv> x - y"
+
+lemma add_nat_eq[simp]: "add_nat = (+)" unfolding add_nat_def by simp
+lemma sub_nat_eq[simp]: "sub_nat = (-)" unfolding sub_nat_def by simp
 
 context includes com_syntax no_com'_syntax
 begin
 
-definition [compiled_const_defs add]:
-  "plus_IMP \<equiv> ''plus_ret'' ::= (V ''plus_x'' \<oplus> V ''plus_y'')"
-definition [compiled_const_defs add]:
-  "minus_IMP \<equiv> ''minus_ret'' ::= (V ''minus_x'' \<ominus> V ''minus_y'')"
+definition [compiled_const_defs]: "add_IMP \<equiv> ''add_ret'' ::= (V ''add_x'' \<oplus> V ''add_y'')"
+definition [compiled_const_defs]: "sub_IMP \<equiv> ''sub_ret'' ::= (V ''sub_x'' \<ominus> V ''sub_y'')"
 
 end
 
-declare_compiled_const "plus_nat"
-  return_register "plus_ret"
-  argument_registers "plus_x" "plus_y"
-  compiled "plus_IMP"
+declare_compiled_const "add_nat"
+  return_register "add_ret"
+  argument_registers "add_x" "add_y"
+  compiled "add_IMP"
 declare_compiled_const "Groups.plus"
-  return_register "plus_ret"
-  argument_registers "plus_x" "plus_y"
-  compiled "plus_IMP"
+  return_register "add_ret"
+  argument_registers "add_x" "add_y"
+  compiled "add_IMP"
 
-declare_compiled_const "minus_nat"
-  return_register "minus_ret"
-  argument_registers "minus_x" "minus_y"
-  compiled "minus_IMP"
+declare_compiled_const "sub_nat"
+  return_register "sub_ret"
+  argument_registers "sub_x" "sub_y"
+  compiled "sub_IMP"
 declare_compiled_const "Groups.minus"
-  return_register "minus_ret"
-  argument_registers "minus_x" "minus_y"
-  compiled "minus_IMP"
+  return_register "sub_ret"
+  argument_registers "sub_x" "sub_y"
+  compiled "sub_IMP"
 
-HOL_To_IMP_Minus_func_correct plus_nat
+HOL_To_IMP_Minus_func_correct add_nat
   by (auto simp: compiled_const_defs)
-HOL_To_IMP_Minus_func_correct minus_nat
+HOL_To_IMP_Minus_func_correct sub_nat
   by (auto simp: compiled_const_defs)
 
 definition max_nat :: "nat \<Rightarrow> nat \<Rightarrow> nat" where
@@ -179,10 +167,7 @@ declare_compiled_const max
   argument_registers "max_x" "max_y"
   compiled "tailcall_to_IMP_Minus max_IMP_tailcall"
 
-HOL_To_IMP_Minus_func_correct max_nat
-  apply preprocess_HOL_To_IMP_Minus_func_correct
-  apply (start_run_finish max_nat_def)
-  done
+HOL_To_IMP_Minus_func_correct max_nat by (cooker HOL_eqs = max_nat_def)
 
 lemma max_nat_eq[simp]: "max_nat x y = max x y"
   unfolding max_nat_def by simp
@@ -197,10 +182,7 @@ declare_compiled_const min
   argument_registers "min_x" "min_y"
   compiled "tailcall_to_IMP_Minus min_IMP_tailcall"
 
-HOL_To_IMP_Minus_func_correct min_nat
-  apply preprocess_HOL_To_IMP_Minus_func_correct
-  apply (start_run_finish min_nat_def)
-  done
+HOL_To_IMP_Minus_func_correct min_nat by (cooker HOL_eqs = min_nat_def)
 
 lemma min_nat_eq[simp]: "min_nat x y = min x y"
   unfolding min_nat_def by simp
@@ -214,10 +196,7 @@ declare_compiled_const conj
   argument_registers "and_x" "and_y"
   compiled "tailcall_to_IMP_Minus and_IMP_tailcall"
 
-HOL_To_IMP_Minus_func_correct and_nat
-  apply preprocess_HOL_To_IMP_Minus_func_correct
-  apply (start_run_finish and_nat_def)
-  done
+HOL_To_IMP_Minus_func_correct and_nat by (cooker HOL_eqs = and_nat_def)
 
 lemma and_nat_eq[simp]: "and_nat x y = nat_of_bool (is_true_nat x \<and> is_true_nat y)"
   unfolding and_nat_def nat_of_bool_def by auto
@@ -231,10 +210,7 @@ declare_compiled_const disj
   argument_registers "or_x" "or_y"
   compiled "tailcall_to_IMP_Minus or_IMP_tailcall"
 
-HOL_To_IMP_Minus_func_correct or_nat
-  apply preprocess_HOL_To_IMP_Minus_func_correct
-  apply (start_run_finish or_nat_def)
-  done
+HOL_To_IMP_Minus_func_correct or_nat by (cooker HOL_eqs = or_nat_def)
 
 lemma or_nat_eq[simp]: "or_nat x y = nat_of_bool (is_true_nat x \<or> is_true_nat y)"
   unfolding or_nat_def nat_of_bool_def by auto
@@ -248,10 +224,7 @@ declare_compiled_const "ord_class.less_eq"
   argument_registers "le_x" "le_y"
   compiled "tailcall_to_IMP_Minus le_IMP_tailcall"
 
-HOL_To_IMP_Minus_func_correct le_nat
-  apply preprocess_HOL_To_IMP_Minus_func_correct
-  apply (start_run_finish le_nat_def)
-  done
+HOL_To_IMP_Minus_func_correct le_nat by (cooker HOL_eqs = le_nat_def)
 
 lemma le_nat_eq[simp]: "le_nat x y = nat_of_bool (x \<le> y)"
   unfolding le_nat_def by simp
@@ -265,10 +238,7 @@ declare_compiled_const "ord_class.less"
   argument_registers "lt_x" "lt_y"
   compiled "tailcall_to_IMP_Minus lt_IMP_tailcall"
 
-HOL_To_IMP_Minus_func_correct lt_nat
-  apply preprocess_HOL_To_IMP_Minus_func_correct
-  apply (start_run_finish lt_nat_def)
-  done
+HOL_To_IMP_Minus_func_correct lt_nat by (cooker HOL_eqs = lt_nat_def)
 
 lemma lt_nat_eq[simp]: "lt_nat x y = nat_of_bool (x < y)"
   unfolding lt_nat_def nat_of_bool_def by auto
