HOL_To_IMP_Minus/Refinements/HOL_To_IMP_Minus_Methods.thy
@@ -4,45 +4,6 @@ theory HOL_To_IMP_Minus_Methods
     HOL_To_IMP_Minus_Goal_Commands
 begin
 
-method preprocess_HOL_To_IMP_Minus_func_correct =
-  (erule tailcall_to_IMP_Minus_correct_if_correct),
-  (subst compiled_const_defs, simp),
-  (subst compiled_const_defs, simp)
-
-method_setup start_run_finish = \<open>
-  let
-    datatype option = Pattern of bool | Induction
-    val option_parser = Parse.group (fn () => "option") (
-      (Parse.reserved "pattern" >> K (Pattern true)) ||
-      (Parse.reserved "no_pattern" >> K (Pattern false)) ||
-      (Parse.reserved "induction" >> K Induction)
-    )
-    val default_options = (false, false)
-    fun apply_option (Pattern b) (_, induction) = (b, induction)
-      | apply_option Induction (pattern, _) = (pattern, true)
-    val options_parser =
-      (Scan.optional (\<^keyword>\<open>(\<close> |-- Parse.!!! (Parse.list1 option_parser) --| \<^keyword>\<open>)\<close>) [])
-      >> (fn opts => fold apply_option opts default_options)
-    val parser = options_parser -- Parse.thm
-  in
-    Scan.lift parser >> (fn ((pattern, induction), fact) => fn ctxt =>
-      let
-        val def_thms = Attrib.eval_thms ctxt [fact]
-        val induction_tac = if induction then H.induction_tac ctxt else K all_tac
-        val run_finish_tac =
-          if pattern
-            then H.start_run_finish_pattern_fun_tac
-            else H.start_run_finish_no_pattern_fun_tac
-        val compiled_const_defs = Named_Theorems.get ctxt \<^named_theorems>\<open>compiled_const_defs\<close>
-        fun correctness_thm_for t =
-          HOL_To_IMP_Minus_Func_Correct_Thms.get_theorem ctxt t
-        val run_finish_tac' =
-          run_finish_tac compiled_const_defs correctness_thm_for def_thms ctxt
-      in
-        SIMPLE_METHOD' (induction_tac THEN_ALL_NEW run_finish_tac')
-      end
-    )
-  end
-\<close>
+fun correctness_thm_for t = HOL_To_IMP_Minus_Func_Correct_Thms.get_theorem ctxt t
 
 end
